\documentclass{article}

\usepackage{fancyhdr}
\usepackage{extramarks}
\usepackage{amsmath}
\usepackage{amsthm}
\usepackage{amsfonts}
\usepackage{tikz}
\usepackage{enumerate}
\usepackage{amssymb}
\usepackage{parskip}
\usepackage{changepage}
\usepackage{autobreak}
\usepackage[UTF8]{ctex}
\usepackage{indentfirst}
\usepackage{algorithm}
\usepackage{algorithmicx}
\usepackage{algpseudocode}

\renewcommand{\algorithmicensure}{\textbf{Initialize:}}
\renewcommand{\algorithmicrequire}{\textbf{Input:}}

\begin{document}

\begin{algorithm}
\caption{UCB-DE}
\begin{algorithmic}[1]
    \Require $\theta_1(\lambda),\theta_2(\lambda),\theta_3(\lambda)$
    \For {$t=1,2,3$}
    \State $I(t)\gets t$
    \State $n_{I(t)}\gets 1$
    \State $\hat{\theta}_{I(t)}\gets r_{I(t)}$
    \EndFor
    \For {$t=4\to N$}
    \State $I^{opt}=\mathop{\arg\max}\limits_{i\in\{1,2,3\}}n_i$
    \State $\Lambda=\left\{\lambda:|\theta_{I^{opt}}(\lambda)-\hat{\theta}({I^{opt}})|\leqslant\sqrt{\frac{2\ln(t)}{n_{I^{opt}}}}\right\}$
    \State $\mathcal{C}=\left\{j:\theta_j(\lambda)=\max\limits_{i\in\{1,2,3\}}\theta_i(\lambda)\text{ for some }\lambda\in(0,1)\right\}$
    \State $I(t)\gets\mathop{\arg\max}\limits_{i\in\mathcal{C}}\left(\hat{\theta}_i+c\sqrt{\frac{2\ln(t)}{n_i}}\right)$
    \State $n_{I(t)}\gets n_{I(t)}+1$
    \State $\hat{\theta}_{I(t)}\gets\hat{\theta}_{I(t)}+\frac{r_{I(t)}-\hat{\theta}_{I(t)}}{n_{I(t)}}$
    \EndFor
\end{algorithmic}
\end{algorithm}

\begin{algorithm}
\caption{UCB-LB}
\begin{algorithmic}[1]
    \Ensure Sort arms in ascending order of cost.
    \State $W_1=W$
    \For {$t=1,2,3$}
    \State $I(t)\gets t$
    \State $n_{I(t)}\gets 1$
    \State $\hat{\theta}_{I(t)}\gets r_{I(t)}$
    \State $W_{t+1}=W_t-c_{I(t)}$
    \EndFor
    \For {$t=4\to N$}
    \State $\mathcal{S}=\Big\{i:c_i\leqslant W_t,i\in\{1,2,3\}\Big\}$
    \If {$\mathcal{S}=\varnothing$}
    \State Terminate the algorithm
    \EndIf
    \State $I(t)\gets\mathop{\arg\max}\limits_{i\in\mathcal{S}}\left(\frac{\hat{\theta}_i+C\sqrt{\frac{2\ln(t)}{n_i}}}{c_i}\right)$
    \State $n_{I(t)}\gets n_{I(t)}+1$
    \State $\hat{\theta}_{I(t)}\gets\hat{\theta}_{I(t)}+\frac{r_{I(t)}-\hat{\theta}_{I(t)}}{n_{I(t)}}$
    \State $W_{t+1}=W_t-c_{I(t)}$
    \EndFor
\end{algorithmic}
\end{algorithm}


\end{document}